\documentclass[a5paper,10pt]{article}

% https://github.com/InDevRus/filippov-solutions
\input{../preambles/general}

\begin{document}

$Cy = \sin\br{Cx}$.
$C y' = C\cos \br{Cx}$.
$y' = \cos\br{Cx}$.
$1 - C^2 y^2 = 1 - \sin^2\br{Cx} = \cos^2\br{Cx} = \linebreak = \br{y'}^2$.
$C^2 =  \dfrac {\br{1 - \br{y'}^2}} {y^2}$.
$y' = \cos\br{Cx} 
= \cos \br{ \vbr{C} x}
= \cos\br{x \sqrt{C^2}}
= \cos\hspace{1mm}\br{\dfrac {x \sqrt{1 - \br{y'}^2}}{y}}$.
Итак, $y' = \cos\hspace{1mm}\br{\dfrac {x \sqrt{1 - \br{y'}^2}}{y}}$.

\end{document}
