\documentclass[a5paper,10pt]{article}

% https://github.com/InDevRus/filippov-solutions
\input{../preambles/general}

\begin{document}

$y = ax^2 + b e^{x}$.
$y' = 2a x + b e^{x}$.
$y'' = 2 a + b e^{x}$.
$b e^{x} = y'' - 2a$.
Подставив в первые два, получим
$\tsys{& y = ax^2 + y'' - 2a \\& y' = 2ax + y '' - 2a}$.
$a = \dfrac {y - y''} {x^2 - 2}$.
$y' = y'' + 2 \br{x - 1} \dfrac {y - y''} {x^2 - 2}$. \\
$x^2y'' - 2y'' - x^2y' + 2y' + 2xy - 2xy'' - 2y + 2y'' = 0$. \\
$y''\br{x^2 - 2x} + \br{2 - x^2}y' + \br{2x - 2}y = 0$.

\end{document}

