\documentclass[a5paper,10pt]{article}

% https://github.com/InDevRus/filippov-solutions
\input{../preambles/general}

\begin{document}

$\ln y = ax + by$.
$b = \dfrac {\ln y - ax} {y}$.
$$0 = \br{\dfrac {\ln y - ax} {y}}'
= \dfrac { \br{\frac {y'}{y} - a}y - \br{\ln y - ax}y'} {y^2}
= \dfrac {y'\br{1 - \ln y + ax} - ay} {y^2}; 
a = \dfrac {y'\br{\ln y - 1}} {xy' - y}.$$
$$0 = \dfrac {\br{y''\br{\ln y - 1} + \frac {\br{y'}^2} {y}}\br{xy' - y} - y'\br{\ln y - 1}\br{y' + xy'' - y'}} {\br{xy' - y}^2}.$$
$xy'y''\br{\ln y - 1} + \dfrac {x\br{y'}^3} {y} - yy''\br{\ln y - 1} - \br{y'}^2 - x y' y''\br{\ln y - 1} = 0$. \\
$y^2 y'' \br{\ln y - 1} = \br{y'}^2 \br{xy' - y}$.

\end{document}

