\documentclass[a5paper,10pt]{article}

% https://github.com/InDevRus/filippov-solutions
\input{../preambles/general}

\begin{document}

$y = ax^3 + bx^2 + cx$.
$y' = 3ax^2 + 2bx + c$.
$c = y' - 3ax^2 - 2bx$. Подставив, получим
$y = ax^3 + bx^2 + xy' - 3ax^3 - 2bx^2$.
$\tsys{& y = -2ax^3 - bx^2 + xy' \\& y' = -6ax^2 - 2bx + y' + xy''}$. \\
$2y = -4ax^3 - 2bx \cdot x + 2xy'
= -4ax^3 + 2xy' - x\br{xy'' - 6ax^2} = 2ax^3 + 2xy' - x^2y''$. \\
$\tsys{& 2y = 2ax^3 + 2xy' - x^2y'' \\& 2y' = 6ax^2 + 2y' + 2xy'' - 2xy'' - x^2y'''}$.
$6a = y'''$.
$6y = x^3 y''' + 6xy' - 3x^2 y'' = 0$.

Итак, $x^3 y''' - 3x^2 y'' + 6xy' - 6y = 0$.

\end{document}

