\documentclass[a5paper,10pt]{article}

% https://github.com/InDevRus/filippov-solutions
\input{../preambles/general}

\begin{document}

$x = ay^2\br{x} + by\br{x} + c$.
$1 = 2ayy' + by'$.
$b = \dfrac {1 - 2ayy'} {y'}$.
\begin{align*}
0 = \dfrac {\br{-2a\br{y'}^2 - 2ayy''}y' - \br{1 - 2ayy'} y''} {\br{y'}^2};
-2a\br{y'}^3 - 2ayy'y'' - y'' + 2ayy'y'' = 0.
\end{align*}
$2a\br{y'}^3 + y'' = 0$.
$a = - \dfrac {y''} {2\br{y'}^3}$.  
$0 = - \dfrac {2y'''\br{y'}^3 - 6\br{y'y''}^2} {2\br{y'}^3}$.
$y'y''' = 3\br{y''}^2$.

\end{document}

