\documentclass[a5paper,10pt]{article}

% https://github.com/InDevRus/filippov-solutions
\input{../preambles/general}

\begin{document}

$\tsys{& ax + \zed = b \\& y^2 + \zed^2 = b^2}$,
где $\tsys{& y = y\br{x} \\& \zed = \zed\br{x}}$.
Продифференцировав первое, имеем $a + \zed' = 0$. \\
$\tsys{& \zed - x\zed' = b \\& y^2 + \zed^2 = b^2}$.
$y^2 + \zed^2 = \br{\zed - x\zed'}^2$.
$y^2 + 2x\zed\zed' - x^2 \br{\zed'}^2 = 0$.
Дифференцирование второго уравнения даёт $yy' + \zed\zed' = 0$.

Окончательно получаем
$\tsys{
	& y^2 + 2x\zed\zed' - x^2 \br{\zed'}^2 = 0 
	\\& yy' + \zed\zed' = 0
}$.

\end{document}

