\documentclass[a5paper,10pt]{article}

% https://github.com/InDevRus/filippov-solutions
\input{../preambles/general}

\begin{document}

$\tsys{
	& x^2 + y^2 = \zed^2 - 2b\zed 
	\\& y = ax + b}$,
где $\tsys{& y = y\br{x} \\& \zed = \zed\br{x}}$.
Продифференцировав второе, имеем $y' = a$. \\
$y = xy' + b$.
$x^2 + y^2 = \zed^2 - 2\zed\br{y - xy'}$.
$x^2 + y^2 - \zed^2 + 2y\zed + 2x\zed y' = 0$.
Далее берём производную первого. $2b = \dfrac {\zed^2 - x^2 - y^2} {\zed}$. \vspace{1mm}
$0 = \dfrac {\br{2\zed\zed' - 2yy' - 2x}\zed - \br{\zed^2 - x^2 - y^2}\zed'} {\zed^2}$. \\
$\zed^2 \zed' - 2y\zed y' - 2x\zed + x^2 \zed' + y^2\zed' = 0$.

Окончательно получаем
$\tsys{
	& x^2 + y^2 - \zed^2 + 2y\zed + 2x\zed y' = 0
	\\& \zed^2 \zed' - 2y\zed y' - 2x\zed + x^2 \zed' + y^2\zed' = 0
}$.

\end{document}

