% Page setup
\documentclass[a5paper,10pt]{article}

% https://github.com/InDevRus/filippov-solutions
\input{../preambles/general}

\begin{document}

$
\begin{cases}
    x'' + 3y'' - x = 0 \\
    x' + 3y' - 2y = 0
\end{cases}
$

$3y' = 2y - x'$. $3y'' = 2y' - x'' = x - x''$, откуда $x = 2y'$. Подставив во второе, получим $2y'' + 3y' - 2y = 0$. $2\lambda^2 + 3\lambda  - 2 = 0$. $\lambda_1 = {-2}, \lambda_{2} = \dfrac {1} {2}$. $y\br{t} = C_{1}  e^{\frac {1} {2} t} + C_{2} e^{-2t}$. $x = 2y' = \linebreak = C_{1}  e^{\frac {1} {2} t} - 4 C_{2} e^{-2t}$.

$
\begin{cases}
    x\br{t} = C_{1}  e^{\frac {1} {2} t} - 4 C_{2} e^{-2t}\\
    y\br{t} = C_{1}  e^{\frac {1} {2} t} + C_{2} e^{-2t}
\end{cases}
$

\end{document}
